examples/rv/RVCore.v
@@ -827,8 +827,7 @@ Module RVCore (RVP: RVParams) (ShadowStack: ShadowStackInterface).
   Definition execute_1
     `{finite_reg: FiniteType reg_t}
     `{finite_reg_stack: FiniteType ShadowStack.reg_t}
-    : uaction reg_t ext_fn_t := {{(
-
+  : uaction reg_t ext_fn_t := {{(
     let fInst      := get(dInst, inst) in
     let funct3     := get(getFields(fInst), funct3) in
     let rd_val     := get(dInst, inst)[|5`d7| :+ 5] in
@@ -895,8 +894,7 @@ Module RVCore (RVP: RVParams) (ShadowStack: ShadowStackInterface).
     `
     else
       pass
-;
-
+    ;
     let controlResult := execControl32(fInst, rs1_val, rs2_val, imm, pc) in
     let nextPc        := get(controlResult,nextPC) in
     if nextPc != get(decoded_bookkeeping, ppc) then
